TheoryTask/qcp-binary-democases/SeparationLogic/examples/sll_project_goal.v
@@ -455,112 +455,43 @@ forall (pt: Z) (l: (@list Z)) (box: Z) ,
 (*----- Function map_list_box -----*)
 
 Definition map_list_box_return_wit_1 := 
-forall (x_pre: Z) (box_pre: Z) (pt: Z) (l: (@list Z)) (h: Z) ,
-  [| (box_pre <> 0) |] 
-  &&  [| (pt = &((box_pre)  # "sllb" ->ₛ "head")) |] 
-  &&  [| (l = nil) |]
+forall (x_pre: Z) (box_pre: Z) (l: (@list Z)) (h: Z) ,
+  [| (box_pre <> 0) |]
   &&  (sll h (map_mult (x_pre) (l)) )
   **  ((&((box_pre)  # "sllb" ->ₛ "head")) # Ptr  |-> h)
-  **  ((&((box_pre)  # "sllb" ->ₛ "ptail")) # Ptr  |-> pt)
+  **  ((&((box_pre)  # "sllb" ->ₛ "ptail")) # Ptr  |-> 0)
 |--
-  EX (pt_new: Z) ,
-  [| (box_pre <> 0) |]
-  &&  ((&((box_pre)  # "sllb" ->ₛ "ptail")) # Ptr  |-> pt_new)
-  **  (sllbseg &((box_pre)  # "sllb" ->ₛ "head") pt_new (map_mult (x_pre) (l)) )
-  **  ((pt_new) # Ptr  |-> 0)
-.
-
-Definition map_list_box_return_wit_2 := 
-forall (x_pre: Z) (box_pre: Z) (pt: Z) (l: (@list Z)) (h: Z) ,
-  [| (box_pre <> 0) |] 
-  &&  [| (pt <> &((box_pre)  # "sllb" ->ₛ "head")) |] 
-  &&  [| (l <> nil) |]
-  &&  (sll h (map_mult (x_pre) (l)) )
-  **  ((&((box_pre)  # "sllb" ->ₛ "head")) # Ptr  |-> h)
-  **  ((&((box_pre)  # "sllb" ->ₛ "ptail")) # Ptr  |-> pt)
-|--
-  EX (pt_new: Z) ,
-  [| (box_pre <> 0) |]
-  &&  ((&((box_pre)  # "sllb" ->ₛ "ptail")) # Ptr  |-> pt_new)
-  **  (sllbseg &((box_pre)  # "sllb" ->ₛ "head") pt_new (map_mult (x_pre) (l)) )
-  **  ((pt_new) # Ptr  |-> 0)
+  (sllb_sll box_pre (map_mult (x_pre) (l)) )
 .
 
 Definition map_list_box_partial_solve_wit_1 := 
-forall (box_pre: Z) (pt: Z) (l: (@list Z)) ,
-  [| (box_pre <> 0) |] 
-  &&  [| (pt = &((box_pre)  # "sllb" ->ₛ "head")) |] 
-  &&  [| (l = nil) |]
-  &&  ((&((box_pre)  # "sllb" ->ₛ "ptail")) # Ptr  |-> pt)
-  **  (sllbseg &((box_pre)  # "sllb" ->ₛ "head") pt l )
-  **  ((pt) # Ptr  |-> 0)
+forall (box_pre: Z) (l: (@list Z)) ,
+  (sllb_sll box_pre l )
 |--
-  [| (box_pre <> 0) |] 
-  &&  [| (pt = &((box_pre)  # "sllb" ->ₛ "head")) |] 
-  &&  [| (l = nil) |]
-  &&  (sllbseg &((box_pre)  # "sllb" ->ₛ "head") pt l )
-  **  ((pt) # Ptr  |-> 0)
-  **  ((&((box_pre)  # "sllb" ->ₛ "ptail")) # Ptr  |-> pt)
+  (sllb_sll box_pre l )
 .
 
 Definition map_list_box_partial_solve_wit_2 := 
-forall (box_pre: Z) (pt: Z) (l: (@list Z)) ,
-  [| (box_pre <> 0) |] 
-  &&  [| (pt <> &((box_pre)  # "sllb" ->ₛ "head")) |] 
-  &&  [| (l <> nil) |]
-  &&  ((&((box_pre)  # "sllb" ->ₛ "ptail")) # Ptr  |-> pt)
-  **  (sllbseg &((box_pre)  # "sllb" ->ₛ "head") pt l )
-  **  ((pt) # Ptr  |-> 0)
-|--
-  [| (box_pre <> 0) |] 
-  &&  [| (pt <> &((box_pre)  # "sllb" ->ₛ "head")) |] 
-  &&  [| (l <> nil) |]
-  &&  (sllbseg &((box_pre)  # "sllb" ->ₛ "head") pt l )
-  **  ((pt) # Ptr  |-> 0)
-  **  ((&((box_pre)  # "sllb" ->ₛ "ptail")) # Ptr  |-> pt)
-.
-
-Definition map_list_box_partial_solve_wit_3 := 
-forall (box_pre: Z) (pt: Z) (l: (@list Z)) (h: Z) ,
-  [| (box_pre <> 0) |] 
-  &&  [| (pt <> &((box_pre)  # "sllb" ->ₛ "head")) |] 
-  &&  [| (l <> nil) |]
+forall (box_pre: Z) (l: (@list Z)) (h: Z) ,
+  [| (box_pre <> 0) |]
   &&  ((&((box_pre)  # "sllb" ->ₛ "head")) # Ptr  |-> h)
+  **  ((&((box_pre)  # "sllb" ->ₛ "ptail")) # Ptr  |-> 0)
   **  (sll h l )
-  **  ((&((box_pre)  # "sllb" ->ₛ "ptail")) # Ptr  |-> pt)
 |--
-  [| (box_pre <> 0) |] 
-  &&  [| (pt <> &((box_pre)  # "sllb" ->ₛ "head")) |] 
-  &&  [| (l <> nil) |]
+  [| (box_pre <> 0) |]
   &&  (sll h l )
   **  ((&((box_pre)  # "sllb" ->ₛ "head")) # Ptr  |-> h)
-  **  ((&((box_pre)  # "sllb" ->ₛ "ptail")) # Ptr  |-> pt)
-.
-
-Definition map_list_box_partial_solve_wit_4 := 
-forall (box_pre: Z) (pt: Z) (l: (@list Z)) (h: Z) ,
-  [| (box_pre <> 0) |] 
-  &&  [| (pt = &((box_pre)  # "sllb" ->ₛ "head")) |] 
-  &&  [| (l = nil) |]
-  &&  ((&((box_pre)  # "sllb" ->ₛ "head")) # Ptr  |-> h)
-  **  (sll h l )
-  **  ((&((box_pre)  # "sllb" ->ₛ "ptail")) # Ptr  |-> pt)
-|--
-  [| (box_pre <> 0) |] 
-  &&  [| (pt = &((box_pre)  # "sllb" ->ₛ "head")) |] 
-  &&  [| (l = nil) |]
-  &&  (sll h l )
-  **  ((&((box_pre)  # "sllb" ->ₛ "head")) # Ptr  |-> h)
-  **  ((&((box_pre)  # "sllb" ->ₛ "ptail")) # Ptr  |-> pt)
+  **  ((&((box_pre)  # "sllb" ->ₛ "ptail")) # Ptr  |-> 0)
 .
 
 Definition map_list_box_which_implies_wit_1 := 
-forall (pt: Z) (l: (@list Z)) (box: Z) ,
-  (sllbseg &((box)  # "sllb" ->ₛ "head") pt l )
-  **  ((pt) # Ptr  |-> 0)
+forall (l: (@list Z)) (box: Z) ,
+  (sllb_sll box l )
 |--
   EX (h: Z) ,
-  ((&((box)  # "sllb" ->ₛ "head")) # Ptr  |-> h)
+  [| (box <> 0) |]
+  &&  ((&((box)  # "sllb" ->ₛ "head")) # Ptr  |-> h)
+  **  ((&((box)  # "sllb" ->ₛ "ptail")) # Ptr  |-> 0)
   **  (sll h l )
 .
 
@@ -1146,198 +1077,74 @@ forall (head_pre: Z) (l: (@list Z)) (l2: (@list Z)) (l1: (@list Z)) (p: Z) (i: Z
 (*----- Function sllb2array -----*)
 
 Definition sllb2array_return_wit_1 := 
-forall (out_array_pre: Z) (box_pre: Z) (out: Z) (b: Z) (pt: Z) (l: (@list Z)) (h: Z) (arr_ret_2: Z) ,
-  [| (b = box_pre) |] 
-  &&  [| (out = out_array_pre) |] 
-  &&  [| (box_pre <> 0) |] 
-  &&  [| ((Zlength (l)) <= INT_MAX) |] 
-  &&  [| (pt <> &((box_pre)  # "sllb" ->ₛ "head")) |] 
-  &&  [| (l <> nil) |]
+forall (out_array_pre: Z) (box_pre: Z) (l: (@list Z)) (h: Z) (arr_ret_2: Z) ,
+  [| (box_pre <> 0) |] 
+  &&  [| ((Zlength (l)) <= INT_MAX) |]
   &&  (sll h l )
   **  ((out_array_pre) # Ptr  |-> arr_ret_2)
   **  (UIntArray.full_shape arr_ret_2 (Zlength (l)) )
   **  ((&((box_pre)  # "sllb" ->ₛ "head")) # Ptr  |-> h)
-  **  ((&((box_pre)  # "sllb" ->ₛ "ptail")) # Ptr  |-> pt)
+  **  ((&((box_pre)  # "sllb" ->ₛ "ptail")) # Ptr  |-> 0)
 |--
-  EX (arr_ret: Z)  (pt_new: Z) ,
-  ((&((b)  # "sllb" ->ₛ "ptail")) # Ptr  |-> pt_new)
-  **  (sllbseg &((b)  # "sllb" ->ₛ "head") pt_new l )
-  **  ((pt_new) # Ptr  |-> 0)
-  **  ((out) # Ptr  |-> arr_ret)
-  **  (UIntArray.full_shape arr_ret (Zlength (l)) )
-.
-
-Definition sllb2array_return_wit_2 := 
-forall (out_array_pre: Z) (box_pre: Z) (out: Z) (b: Z) (pt: Z) (l: (@list Z)) (h: Z) (arr_ret_2: Z) ,
-  [| (b = box_pre) |] 
-  &&  [| (out = out_array_pre) |] 
-  &&  [| (box_pre <> 0) |] 
-  &&  [| ((Zlength (l)) <= INT_MAX) |] 
-  &&  [| (pt = &((box_pre)  # "sllb" ->ₛ "head")) |] 
-  &&  [| (l = nil) |]
-  &&  (sll h l )
-  **  ((out_array_pre) # Ptr  |-> arr_ret_2)
-  **  (UIntArray.full_shape arr_ret_2 (Zlength (l)) )
-  **  ((&((box_pre)  # "sllb" ->ₛ "head")) # Ptr  |-> h)
-  **  ((&((box_pre)  # "sllb" ->ₛ "ptail")) # Ptr  |-> pt)
-|--
-  EX (arr_ret: Z)  (pt_new: Z) ,
-  ((&((b)  # "sllb" ->ₛ "ptail")) # Ptr  |-> pt_new)
-  **  (sllbseg &((b)  # "sllb" ->ₛ "head") pt_new l )
-  **  ((pt_new) # Ptr  |-> 0)
-  **  ((out) # Ptr  |-> arr_ret)
+  EX (arr_ret: Z) ,
+  (sllb_sll box_pre l )
+  **  ((out_array_pre) # Ptr  |-> arr_ret)
   **  (UIntArray.full_shape arr_ret (Zlength (l)) )
 .
 
 Definition sllb2array_partial_solve_wit_1 := 
-forall (out_array_pre: Z) (box_pre: Z) (out: Z) (b: Z) (pt: Z) (l: (@list Z)) ,
-  [| (b = box_pre) |] 
-  &&  [| (out = out_array_pre) |] 
-  &&  [| (box_pre <> 0) |] 
-  &&  [| ((Zlength (l)) <= INT_MAX) |] 
-  &&  [| (pt = &((box_pre)  # "sllb" ->ₛ "head")) |] 
-  &&  [| (l = nil) |]
-  &&  ((&((box_pre)  # "sllb" ->ₛ "ptail")) # Ptr  |-> pt)
-  **  (sllbseg &((box_pre)  # "sllb" ->ₛ "head") pt l )
-  **  ((pt) # Ptr  |-> 0)
+forall (out_array_pre: Z) (box_pre: Z) (l: (@list Z)) ,
+  [| ((Zlength (l)) <= INT_MAX) |]
+  &&  (sllb_sll box_pre l )
   **  ((out_array_pre) # Ptr  |->_)
 |--
-  [| (b = box_pre) |] 
-  &&  [| (out = out_array_pre) |] 
-  &&  [| (box_pre <> 0) |] 
-  &&  [| ((Zlength (l)) <= INT_MAX) |] 
-  &&  [| (pt = &((box_pre)  # "sllb" ->ₛ "head")) |] 
-  &&  [| (l = nil) |]
-  &&  (sllbseg &((box_pre)  # "sllb" ->ₛ "head") pt l )
-  **  ((pt) # Ptr  |-> 0)
-  **  ((&((box_pre)  # "sllb" ->ₛ "ptail")) # Ptr  |-> pt)
+  [| ((Zlength (l)) <= INT_MAX) |]
+  &&  (sllb_sll box_pre l )
   **  ((out_array_pre) # Ptr  |->_)
 .
 
-Definition sllb2array_partial_solve_wit_2 := 
-forall (out_array_pre: Z) (box_pre: Z) (out: Z) (b: Z) (pt: Z) (l: (@list Z)) ,
-  [| (b = box_pre) |] 
-  &&  [| (out = out_array_pre) |] 
-  &&  [| (box_pre <> 0) |] 
-  &&  [| ((Zlength (l)) <= INT_MAX) |] 
-  &&  [| (pt <> &((box_pre)  # "sllb" ->ₛ "head")) |] 
-  &&  [| (l <> nil) |]
-  &&  ((&((box_pre)  # "sllb" ->ₛ "ptail")) # Ptr  |-> pt)
-  **  (sllbseg &((box_pre)  # "sllb" ->ₛ "head") pt l )
-  **  ((pt) # Ptr  |-> 0)
-  **  ((out_array_pre) # Ptr  |->_)
-|--
-  [| (b = box_pre) |] 
-  &&  [| (out = out_array_pre) |] 
-  &&  [| (box_pre <> 0) |] 
-  &&  [| ((Zlength (l)) <= INT_MAX) |] 
-  &&  [| (pt <> &((box_pre)  # "sllb" ->ₛ "head")) |] 
-  &&  [| (l <> nil) |]
-  &&  (sllbseg &((box_pre)  # "sllb" ->ₛ "head") pt l )
-  **  ((pt) # Ptr  |-> 0)
-  **  ((&((box_pre)  # "sllb" ->ₛ "ptail")) # Ptr  |-> pt)
-  **  ((out_array_pre) # Ptr  |->_)
-.
-
-Definition sllb2array_partial_solve_wit_3_pure := 
-forall (out_array_pre: Z) (box_pre: Z) (out: Z) (b: Z) (pt: Z) (l: (@list Z)) (h: Z) ,
-  [| (b = box_pre) |] 
-  &&  [| (out = out_array_pre) |] 
-  &&  [| (box_pre <> 0) |] 
-  &&  [| ((Zlength (l)) <= INT_MAX) |] 
-  &&  [| (pt <> &((box_pre)  # "sllb" ->ₛ "head")) |] 
-  &&  [| (l <> nil) |]
+Definition sllb2array_partial_solve_wit_2_pure := 
+forall (out_array_pre: Z) (box_pre: Z) (l: (@list Z)) (h: Z) ,
+  [| (box_pre <> 0) |] 
+  &&  [| ((Zlength (l)) <= INT_MAX) |]
   &&  ((( &( "box" ) )) # Ptr  |-> box_pre)
   **  ((&((box_pre)  # "sllb" ->ₛ "head")) # Ptr  |-> h)
+  **  ((&((box_pre)  # "sllb" ->ₛ "ptail")) # Ptr  |-> 0)
   **  (sll h l )
   **  ((( &( "out_array" ) )) # Ptr  |-> out_array_pre)
-  **  ((&((box_pre)  # "sllb" ->ₛ "ptail")) # Ptr  |-> pt)
   **  ((out_array_pre) # Ptr  |->_)
 |--
   [| ((Zlength (l)) <= INT_MAX) |]
 .
 
-Definition sllb2array_partial_solve_wit_3_aux := 
-forall (out_array_pre: Z) (box_pre: Z) (out: Z) (b: Z) (pt: Z) (l: (@list Z)) (h: Z) ,
-  [| (b = box_pre) |] 
-  &&  [| (out = out_array_pre) |] 
-  &&  [| (box_pre <> 0) |] 
-  &&  [| ((Zlength (l)) <= INT_MAX) |] 
-  &&  [| (pt <> &((box_pre)  # "sllb" ->ₛ "head")) |] 
-  &&  [| (l <> nil) |]
+Definition sllb2array_partial_solve_wit_2_aux := 
+forall (out_array_pre: Z) (box_pre: Z) (l: (@list Z)) (h: Z) ,
+  [| (box_pre <> 0) |] 
+  &&  [| ((Zlength (l)) <= INT_MAX) |]
   &&  ((&((box_pre)  # "sllb" ->ₛ "head")) # Ptr  |-> h)
+  **  ((&((box_pre)  # "sllb" ->ₛ "ptail")) # Ptr  |-> 0)
   **  (sll h l )
-  **  ((&((box_pre)  # "sllb" ->ₛ "ptail")) # Ptr  |-> pt)
   **  ((out_array_pre) # Ptr  |->_)
 |--
   [| ((Zlength (l)) <= INT_MAX) |] 
-  &&  [| (b = box_pre) |] 
-  &&  [| (out = out_array_pre) |] 
   &&  [| (box_pre <> 0) |] 
-  &&  [| ((Zlength (l)) <= INT_MAX) |] 
-  &&  [| (pt <> &((box_pre)  # "sllb" ->ₛ "head")) |] 
-  &&  [| (l <> nil) |]
+  &&  [| ((Zlength (l)) <= INT_MAX) |]
   &&  (sll h l )
   **  ((out_array_pre) # Ptr  |->_)
   **  ((&((box_pre)  # "sllb" ->ₛ "head")) # Ptr  |-> h)
-  **  ((&((box_pre)  # "sllb" ->ₛ "ptail")) # Ptr  |-> pt)
+  **  ((&((box_pre)  # "sllb" ->ₛ "ptail")) # Ptr  |-> 0)
 .
 
-Definition sllb2array_partial_solve_wit_3 := sllb2array_partial_solve_wit_3_pure -> sllb2array_partial_solve_wit_3_aux.
-
-Definition sllb2array_partial_solve_wit_4_pure := 
-forall (out_array_pre: Z) (box_pre: Z) (out: Z) (b: Z) (pt: Z) (l: (@list Z)) (h: Z) ,
-  [| (b = box_pre) |] 
-  &&  [| (out = out_array_pre) |] 
-  &&  [| (box_pre <> 0) |] 
-  &&  [| ((Zlength (l)) <= INT_MAX) |] 
-  &&  [| (pt = &((box_pre)  # "sllb" ->ₛ "head")) |] 
-  &&  [| (l = nil) |]
-  &&  ((( &( "box" ) )) # Ptr  |-> box_pre)
-  **  ((&((box_pre)  # "sllb" ->ₛ "head")) # Ptr  |-> h)
-  **  (sll h l )
-  **  ((( &( "out_array" ) )) # Ptr  |-> out_array_pre)
-  **  ((&((box_pre)  # "sllb" ->ₛ "ptail")) # Ptr  |-> pt)
-  **  ((out_array_pre) # Ptr  |->_)
-|--
-  [| ((Zlength (l)) <= INT_MAX) |]
-.
-
-Definition sllb2array_partial_solve_wit_4_aux := 
-forall (out_array_pre: Z) (box_pre: Z) (out: Z) (b: Z) (pt: Z) (l: (@list Z)) (h: Z) ,
-  [| (b = box_pre) |] 
-  &&  [| (out = out_array_pre) |] 
-  &&  [| (box_pre <> 0) |] 
-  &&  [| ((Zlength (l)) <= INT_MAX) |] 
-  &&  [| (pt = &((box_pre)  # "sllb" ->ₛ "head")) |] 
-  &&  [| (l = nil) |]
-  &&  ((&((box_pre)  # "sllb" ->ₛ "head")) # Ptr  |-> h)
-  **  (sll h l )
-  **  ((&((box_pre)  # "sllb" ->ₛ "ptail")) # Ptr  |-> pt)
-  **  ((out_array_pre) # Ptr  |->_)
-|--
-  [| ((Zlength (l)) <= INT_MAX) |] 
-  &&  [| (b = box_pre) |] 
-  &&  [| (out = out_array_pre) |] 
-  &&  [| (box_pre <> 0) |] 
-  &&  [| ((Zlength (l)) <= INT_MAX) |] 
-  &&  [| (pt = &((box_pre)  # "sllb" ->ₛ "head")) |] 
-  &&  [| (l = nil) |]
-  &&  (sll h l )
-  **  ((out_array_pre) # Ptr  |->_)
-  **  ((&((box_pre)  # "sllb" ->ₛ "head")) # Ptr  |-> h)
-  **  ((&((box_pre)  # "sllb" ->ₛ "ptail")) # Ptr  |-> pt)
-.
-
-Definition sllb2array_partial_solve_wit_4 := sllb2array_partial_solve_wit_4_pure -> sllb2array_partial_solve_wit_4_aux.
+Definition sllb2array_partial_solve_wit_2 := sllb2array_partial_solve_wit_2_pure -> sllb2array_partial_solve_wit_2_aux.
 
 Definition sllb2array_which_implies_wit_1 := 
-forall (pt: Z) (l: (@list Z)) (box: Z) ,
-  (sllbseg &((box)  # "sllb" ->ₛ "head") pt l )
-  **  ((pt) # Ptr  |-> 0)
+forall (l: (@list Z)) (box: Z) ,
+  (sllb_sll box l )
 |--
   EX (h: Z) ,
-  ((&((box)  # "sllb" ->ₛ "head")) # Ptr  |-> h)
+  [| (box <> 0) |]
+  &&  ((&((box)  # "sllb" ->ₛ "head")) # Ptr  |-> h)
+  **  ((&((box)  # "sllb" ->ₛ "ptail")) # Ptr  |-> 0)
   **  (sll h l )
 .
 
@@ -1379,11 +1186,8 @@ Axiom proof_of_cons_list_box_partial_solve_wit_3 : cons_list_box_partial_solve_w
 Axiom proof_of_cons_list_box_partial_solve_wit_4 : cons_list_box_partial_solve_wit_4.
 Axiom proof_of_cons_list_box_which_implies_wit_1 : cons_list_box_which_implies_wit_1.
 Axiom proof_of_map_list_box_return_wit_1 : map_list_box_return_wit_1.
-Axiom proof_of_map_list_box_return_wit_2 : map_list_box_return_wit_2.
 Axiom proof_of_map_list_box_partial_solve_wit_1 : map_list_box_partial_solve_wit_1.
 Axiom proof_of_map_list_box_partial_solve_wit_2 : map_list_box_partial_solve_wit_2.
-Axiom proof_of_map_list_box_partial_solve_wit_3 : map_list_box_partial_solve_wit_3.
-Axiom proof_of_map_list_box_partial_solve_wit_4 : map_list_box_partial_solve_wit_4.
 Axiom proof_of_map_list_box_which_implies_wit_1 : map_list_box_which_implies_wit_1.
 Axiom proof_of_free_list_box_return_wit_1 : free_list_box_return_wit_1.
 Axiom proof_of_free_list_box_partial_solve_wit_1 : free_list_box_partial_solve_wit_1.
@@ -1418,13 +1222,9 @@ Axiom proof_of_sll2array_partial_solve_wit_3 : sll2array_partial_solve_wit_3.
 Axiom proof_of_sll2array_partial_solve_wit_4 : sll2array_partial_solve_wit_4.
 Axiom proof_of_sll2array_which_implies_wit_1 : sll2array_which_implies_wit_1.
 Axiom proof_of_sllb2array_return_wit_1 : sllb2array_return_wit_1.
-Axiom proof_of_sllb2array_return_wit_2 : sllb2array_return_wit_2.
 Axiom proof_of_sllb2array_partial_solve_wit_1 : sllb2array_partial_solve_wit_1.
+Axiom proof_of_sllb2array_partial_solve_wit_2_pure : sllb2array_partial_solve_wit_2_pure.
 Axiom proof_of_sllb2array_partial_solve_wit_2 : sllb2array_partial_solve_wit_2.
-Axiom proof_of_sllb2array_partial_solve_wit_3_pure : sllb2array_partial_solve_wit_3_pure.
-Axiom proof_of_sllb2array_partial_solve_wit_3 : sllb2array_partial_solve_wit_3.
-Axiom proof_of_sllb2array_partial_solve_wit_4_pure : sllb2array_partial_solve_wit_4_pure.
-Axiom proof_of_sllb2array_partial_solve_wit_4 : sllb2array_partial_solve_wit_4.
 Axiom proof_of_sllb2array_which_implies_wit_1 : sllb2array_which_implies_wit_1.
 
 End VC_Correct.
